backend/Allocation.v
@@ -116,8 +116,7 @@ Module RegsetLat := LFSet(Regset).
 Module DS := Backward_Dataflow_Solver(RegsetLat)(NodeSetBackward).
 
 Section WITHEF.
-Require Import ExtFunImpl.
-Existing Instances ef_ops sc_ops ef_spec.
+Context `{Hsc: SyntaxConfiguration}.
 
 Definition analyze (f: RTL.function): option (PMap.t Regset.t) :=
   DS.fixpoint (successors f)  (transfer f) nil.
